chore(core-models): regenerate the extraction and coverage for the large-core group

hax-lib/proof-libs/fstar/core/Core_models.Slice.Iter.fst
@@ -3,6 +3,52 @@ module Core_models.Slice.Iter
 open FStar.Mul
 open Rust_primitives
 
+/// Index of the first element of `s` satisfying `pred`, or `s.len()` if
+/// there is none. A bounded loop with no early exit, which is the shape both
+/// backends handle; `pred` is taken by reference so the split iterators can
+/// call it out of `&mut self`.
+assume
+val position_of':
+    #v_T: Type0 ->
+    #v_P: Type0 ->
+    {| i0: Core_models.Ops.Function.t_Fn v_P v_T |} ->
+    s: t_Slice v_T ->
+    pred: v_P
+  -> Prims.Pure usize
+      Prims.l_True
+      (ensures
+        fun res ->
+          let res:usize = res in
+          res <=. (Rust_primitives.Slice.slice_length #v_T s <: usize))
+
+unfold
+let position_of
+      (#v_T #v_P: Type0)
+      (#[FStar.Tactics.Typeclasses.tcresolve ()] i0: Core_models.Ops.Function.t_Fn v_P v_T)
+     = position_of' #v_T #v_P #i0
+
+/// Index of the *last* element of `s` satisfying `pred`, or `s.len()` if
+/// there is none.
+assume
+val rposition_of':
+    #v_T: Type0 ->
+    #v_P: Type0 ->
+    {| i0: Core_models.Ops.Function.t_Fn v_P v_T |} ->
+    s: t_Slice v_T ->
+    pred: v_P
+  -> Prims.Pure usize
+      Prims.l_True
+      (ensures
+        fun res ->
+          let res:usize = res in
+          res <=. (Rust_primitives.Slice.slice_length #v_T s <: usize))
+
+unfold
+let rposition_of
+      (#v_T #v_P: Type0)
+      (#[FStar.Tactics.Typeclasses.tcresolve ()] i0: Core_models.Ops.Function.t_Fn v_P v_T)
+     = rposition_of' #v_T #v_P #i0
+
 /// See [`std::slice::Chunks`]
 type t_Chunks (v_T: Type0) = {
   f_cs:usize;
@@ -15,11 +61,20 @@ let impl__new (#v_T: Type0) (cs: usize) (elements: t_Slice v_T) : t_Chunks v_T =
 /// See [`std::slice::ChunksExact`]
 type t_ChunksExact (v_T: Type0) = {
   f_cs:usize;
-  f_elements:t_Slice v_T
+  f_elements:t_Slice v_T;
+  f_rem:t_Slice v_T
 }
 
 let impl_1__new (#v_T: Type0) (cs: usize) (elements: t_Slice v_T) : t_ChunksExact v_T =
-  { f_cs = cs; f_elements = elements } <: t_ChunksExact v_T
+  let len:usize = Rust_primitives.Slice.slice_length #v_T elements in
+  let rem_len:usize = if cs =. mk_usize 0 then mk_usize 0 else len %! cs in
+  let rem:t_Slice v_T =
+    Rust_primitives.Slice.slice_slice #v_T elements (len -! rem_len <: usize) len
+  in
+  { f_cs = cs; f_elements = elements; f_rem = rem } <: t_ChunksExact v_T
+
+/// See [`std::slice::ChunksExact::remainder`]
+let impl_1__remainder (#v_T: Type0) (self: t_ChunksExact v_T) : t_Slice v_T = self.f_rem
 
 /// See [`std::slice::Iter`]
 type t_Iter (v_T: Type0) = | Iter : Rust_primitives.Sequence.t_Seq v_T -> t_Iter v_T
@@ -151,3 +206,505 @@ val impl_6': #v_T: Type0 -> Core_models.Iter.Traits.Iterator.t_Iterator (t_Windo
 
 unfold
 let impl_6 (#v_T: Type0) = impl_6' #v_T
+
+/// See [`std::slice::RChunks`]
+type t_RChunks (v_T: Type0) = {
+  f_cs:usize;
+  f_elements:t_Slice v_T
+}
+
+let impl_7__new (#v_T: Type0) (cs: usize) (elements: t_Slice v_T) : t_RChunks v_T =
+  { f_cs = cs; f_elements = elements } <: t_RChunks v_T
+
+[@@ FStar.Tactics.Typeclasses.tcinstance]
+let impl_8 (#v_T: Type0) : Core_models.Iter.Traits.Iterator.t_Iterator (t_RChunks v_T) =
+  {
+    f_Item = t_Slice v_T;
+    f_next_pre = (fun (self: t_RChunks v_T) -> true);
+    f_next_post
+    =
+    (fun (self: t_RChunks v_T) (out: (t_RChunks v_T & Core_models.Option.t_Option (t_Slice v_T))) ->
+        true);
+    f_next
+    =
+    fun (self: t_RChunks v_T) ->
+      let len:usize = Rust_primitives.Slice.slice_length #v_T self.f_elements in
+      let (self: t_RChunks v_T), (hax_temp_output: Core_models.Option.t_Option (t_Slice v_T)) =
+        if len =. mk_usize 0
+        then
+          self, (Core_models.Option.Option_None <: Core_models.Option.t_Option (t_Slice v_T))
+          <:
+          (t_RChunks v_T & Core_models.Option.t_Option (t_Slice v_T))
+        else
+          if len <. self.f_cs
+          then
+            let res:t_Slice v_T = self.f_elements in
+            let self:t_RChunks v_T =
+              {
+                self with
+                f_elements
+                =
+                Rust_primitives.Slice.slice_slice #v_T self.f_elements (mk_usize 0) (mk_usize 0)
+              }
+              <:
+              t_RChunks v_T
+            in
+            self, (Core_models.Option.Option_Some res <: Core_models.Option.t_Option (t_Slice v_T))
+            <:
+            (t_RChunks v_T & Core_models.Option.t_Option (t_Slice v_T))
+          else
+            let (rest: t_Slice v_T), (res: t_Slice v_T) =
+              Rust_primitives.Slice.slice_split_at #v_T self.f_elements (len -! self.f_cs <: usize)
+            in
+            let self:t_RChunks v_T = { self with f_elements = rest } <: t_RChunks v_T in
+            self, (Core_models.Option.Option_Some res <: Core_models.Option.t_Option (t_Slice v_T))
+            <:
+            (t_RChunks v_T & Core_models.Option.t_Option (t_Slice v_T))
+      in
+      self, hax_temp_output <: (t_RChunks v_T & Core_models.Option.t_Option (t_Slice v_T))
+  }
+
+/// See [`std::slice::RChunksExact`]
+type t_RChunksExact (v_T: Type0) = {
+  f_cs:usize;
+  f_elements:t_Slice v_T;
+  f_rem:t_Slice v_T
+}
+
+let impl_9__new (#v_T: Type0) (cs: usize) (elements: t_Slice v_T) : t_RChunksExact v_T =
+  let rem_len:usize =
+    if cs =. mk_usize 0
+    then mk_usize 0
+    else (Rust_primitives.Slice.slice_length #v_T elements <: usize) %! cs
+  in
+  let (rem: t_Slice v_T), (els: t_Slice v_T) =
+    Rust_primitives.Slice.slice_split_at #v_T elements rem_len
+  in
+  { f_cs = cs; f_elements = els; f_rem = rem } <: t_RChunksExact v_T
+
+/// See [`std::slice::RChunksExact::remainder`]
+let impl_9__remainder (#v_T: Type0) (self: t_RChunksExact v_T) : t_Slice v_T = self.f_rem
+
+[@@ FStar.Tactics.Typeclasses.tcinstance]
+let impl_10 (#v_T: Type0) : Core_models.Iter.Traits.Iterator.t_Iterator (t_RChunksExact v_T) =
+  {
+    f_Item = t_Slice v_T;
+    f_next_pre = (fun (self: t_RChunksExact v_T) -> true);
+    f_next_post
+    =
+    (fun
+        (self: t_RChunksExact v_T)
+        (out: (t_RChunksExact v_T & Core_models.Option.t_Option (t_Slice v_T)))
+        ->
+        true);
+    f_next
+    =
+    fun (self: t_RChunksExact v_T) ->
+      let len:usize = Rust_primitives.Slice.slice_length #v_T self.f_elements in
+      let (self: t_RChunksExact v_T), (hax_temp_output: Core_models.Option.t_Option (t_Slice v_T)) =
+        if len <. self.f_cs
+        then
+          self, (Core_models.Option.Option_None <: Core_models.Option.t_Option (t_Slice v_T))
+          <:
+          (t_RChunksExact v_T & Core_models.Option.t_Option (t_Slice v_T))
+        else
+          let (rest: t_Slice v_T), (res: t_Slice v_T) =
+            Rust_primitives.Slice.slice_split_at #v_T self.f_elements (len -! self.f_cs <: usize)
+          in
+          let self:t_RChunksExact v_T = { self with f_elements = rest } <: t_RChunksExact v_T in
+          self, (Core_models.Option.Option_Some res <: Core_models.Option.t_Option (t_Slice v_T))
+          <:
+          (t_RChunksExact v_T & Core_models.Option.t_Option (t_Slice v_T))
+      in
+      self, hax_temp_output <: (t_RChunksExact v_T & Core_models.Option.t_Option (t_Slice v_T))
+  }
+
+/// See [`std::slice::Split`]
+type t_Split (v_T: Type0) (v_P: Type0) = {
+  f_v:t_Slice v_T;
+  f_pred:v_P;
+  f_finished:bool
+}
+
+let impl_11__new
+      (#v_T #v_P: Type0)
+      (#[FStar.Tactics.Typeclasses.tcresolve ()] i0: Core_models.Ops.Function.t_Fn v_P v_T)
+      (v: t_Slice v_T)
+      (pred: v_P)
+    : t_Split v_T v_P = { f_v = v; f_pred = pred; f_finished = false } <: t_Split v_T v_P
+
+/// See [`std::slice::Split::as_slice`]
+let impl_11__as_slice
+      (#v_T #v_P: Type0)
+      (#[FStar.Tactics.Typeclasses.tcresolve ()] i0: Core_models.Ops.Function.t_Fn v_P v_T)
+      (self: t_Split v_T v_P)
+    : t_Slice v_T =
+  if self.f_finished
+  then Rust_primitives.Slice.slice_slice #v_T self.f_v (mk_usize 0) (mk_usize 0)
+  else self.f_v
+
+/// Yields the whole remaining slice and stops: what `splitn` does once
+/// its split budget is used up.
+let impl_11__finish
+      (#v_T #v_P: Type0)
+      (#[FStar.Tactics.Typeclasses.tcresolve ()] i0: Core_models.Ops.Function.t_Fn v_P v_T)
+      (self: t_Split v_T v_P)
+    : (t_Split v_T v_P & Core_models.Option.t_Option (t_Slice v_T)) =
+  let (self: t_Split v_T v_P), (hax_temp_output: Core_models.Option.t_Option (t_Slice v_T)) =
+    if self.f_finished
+    then
+      self, (Core_models.Option.Option_None <: Core_models.Option.t_Option (t_Slice v_T))
+      <:
+      (t_Split v_T v_P & Core_models.Option.t_Option (t_Slice v_T))
+    else
+      let self:t_Split v_T v_P = { self with f_finished = true } <: t_Split v_T v_P in
+      self, (Core_models.Option.Option_Some self.f_v <: Core_models.Option.t_Option (t_Slice v_T))
+      <:
+      (t_Split v_T v_P & Core_models.Option.t_Option (t_Slice v_T))
+  in
+  self, hax_temp_output <: (t_Split v_T v_P & Core_models.Option.t_Option (t_Slice v_T))
+
+/// The `DoubleEndedIterator` half of `Split`, which is all `RSplit` is.
+let impl_11__next_back
+      (#v_T #v_P: Type0)
+      (#[FStar.Tactics.Typeclasses.tcresolve ()] i0: Core_models.Ops.Function.t_Fn v_P v_T)
+      (self: t_Split v_T v_P)
+    : (t_Split v_T v_P & Core_models.Option.t_Option (t_Slice v_T)) =
+  let (self: t_Split v_T v_P), (hax_temp_output: Core_models.Option.t_Option (t_Slice v_T)) =
+    if self.f_finished
+    then
+      self, (Core_models.Option.Option_None <: Core_models.Option.t_Option (t_Slice v_T))
+      <:
+      (t_Split v_T v_P & Core_models.Option.t_Option (t_Slice v_T))
+    else
+      let len:usize = Rust_primitives.Slice.slice_length #v_T self.f_v in
+      let idx:usize = rposition_of #v_T #v_P self.f_v self.f_pred in
+      if idx =. len
+      then
+        let self:t_Split v_T v_P = { self with f_finished = true } <: t_Split v_T v_P in
+        self, (Core_models.Option.Option_Some self.f_v <: Core_models.Option.t_Option (t_Slice v_T))
+        <:
+        (t_Split v_T v_P & Core_models.Option.t_Option (t_Slice v_T))
+      else
+        let res:t_Slice v_T =
+          Rust_primitives.Slice.slice_slice #v_T self.f_v (idx +! mk_usize 1 <: usize) len
+        in
+        let self:t_Split v_T v_P =
+          { self with f_v = Rust_primitives.Slice.slice_slice #v_T self.f_v (mk_usize 0) idx }
+          <:
+          t_Split v_T v_P
+        in
+        self, (Core_models.Option.Option_Some res <: Core_models.Option.t_Option (t_Slice v_T))
+        <:
+        (t_Split v_T v_P & Core_models.Option.t_Option (t_Slice v_T))
+  in
+  self, hax_temp_output <: (t_Split v_T v_P & Core_models.Option.t_Option (t_Slice v_T))
+
+[@@ FStar.Tactics.Typeclasses.tcinstance]
+let impl_12
+      (#v_T #v_P: Type0)
+      (#[FStar.Tactics.Typeclasses.tcresolve ()] i0: Core_models.Ops.Function.t_Fn v_P v_T)
+    : Core_models.Iter.Traits.Iterator.t_Iterator (t_Split v_T v_P) =
+  {
+    f_Item = t_Slice v_T;
+    f_next_pre = (fun (self: t_Split v_T v_P) -> true);
+    f_next_post
+    =
+    (fun
+        (self: t_Split v_T v_P)
+        (out: (t_Split v_T v_P & Core_models.Option.t_Option (t_Slice v_T)))
+        ->
+        true);
+    f_next
+    =
+    fun (self: t_Split v_T v_P) ->
+      let (self: t_Split v_T v_P), (hax_temp_output: Core_models.Option.t_Option (t_Slice v_T)) =
+        if self.f_finished
+        then
+          self, (Core_models.Option.Option_None <: Core_models.Option.t_Option (t_Slice v_T))
+          <:
+          (t_Split v_T v_P & Core_models.Option.t_Option (t_Slice v_T))
+        else
+          let len:usize = Rust_primitives.Slice.slice_length #v_T self.f_v in
+          let idx:usize = position_of #v_T #v_P self.f_v self.f_pred in
+          if idx =. len
+          then
+            let self:t_Split v_T v_P = { self with f_finished = true } <: t_Split v_T v_P in
+            self,
+            (Core_models.Option.Option_Some self.f_v <: Core_models.Option.t_Option (t_Slice v_T))
+            <:
+            (t_Split v_T v_P & Core_models.Option.t_Option (t_Slice v_T))
+          else
+            let res:t_Slice v_T =
+              Rust_primitives.Slice.slice_slice #v_T self.f_v (mk_usize 0) idx
+            in
+            let self:t_Split v_T v_P =
+              {
+                self with
+                f_v
+                =
+                Rust_primitives.Slice.slice_slice #v_T self.f_v (idx +! mk_usize 1 <: usize) len
+              }
+              <:
+              t_Split v_T v_P
+            in
+            self, (Core_models.Option.Option_Some res <: Core_models.Option.t_Option (t_Slice v_T))
+            <:
+            (t_Split v_T v_P & Core_models.Option.t_Option (t_Slice v_T))
+      in
+      self, hax_temp_output <: (t_Split v_T v_P & Core_models.Option.t_Option (t_Slice v_T))
+  }
+
+/// See [`std::slice::SplitInclusive`]
+type t_SplitInclusive (v_T: Type0) (v_P: Type0) = {
+  f_v:t_Slice v_T;
+  f_pred:v_P;
+  f_finished:bool
+}
+
+let impl_13__new
+      (#v_T #v_P: Type0)
+      (#[FStar.Tactics.Typeclasses.tcresolve ()] i0: Core_models.Ops.Function.t_Fn v_P v_T)
+      (v: t_Slice v_T)
+      (pred: v_P)
+    : t_SplitInclusive v_T v_P =
+  let finished:bool = (Rust_primitives.Slice.slice_length #v_T v <: usize) =. mk_usize 0 in
+  { f_v = v; f_pred = pred; f_finished = finished } <: t_SplitInclusive v_T v_P
+
+[@@ FStar.Tactics.Typeclasses.tcinstance]
+let impl_14
+      (#v_T #v_P: Type0)
+      (#[FStar.Tactics.Typeclasses.tcresolve ()] i0: Core_models.Ops.Function.t_Fn v_P v_T)
+    : Core_models.Iter.Traits.Iterator.t_Iterator (t_SplitInclusive v_T v_P) =
+  {
+    f_Item = t_Slice v_T;
+    f_next_pre = (fun (self: t_SplitInclusive v_T v_P) -> true);
+    f_next_post
+    =
+    (fun
+        (self: t_SplitInclusive v_T v_P)
+        (out: (t_SplitInclusive v_T v_P & Core_models.Option.t_Option (t_Slice v_T)))
+        ->
+        true);
+    f_next
+    =
+    fun (self: t_SplitInclusive v_T v_P) ->
+      let
+      (self: t_SplitInclusive v_T v_P), (hax_temp_output: Core_models.Option.t_Option (t_Slice v_T))
+      =
+        if self.f_finished
+        then
+          self, (Core_models.Option.Option_None <: Core_models.Option.t_Option (t_Slice v_T))
+          <:
+          (t_SplitInclusive v_T v_P & Core_models.Option.t_Option (t_Slice v_T))
+        else
+          let len:usize = Rust_primitives.Slice.slice_length #v_T self.f_v in
+          let p:usize = position_of #v_T #v_P self.f_v self.f_pred in
+          let idx:usize = if p =. len then len else p +! mk_usize 1 in
+          let self:t_SplitInclusive v_T v_P =
+            if idx =. len
+            then
+              let self:t_SplitInclusive v_T v_P =
+                { self with f_finished = true } <: t_SplitInclusive v_T v_P
+              in
+              self
+            else self
+          in
+          let res:t_Slice v_T = Rust_primitives.Slice.slice_slice #v_T self.f_v (mk_usize 0) idx in
+          let self:t_SplitInclusive v_T v_P =
+            { self with f_v = Rust_primitives.Slice.slice_slice #v_T self.f_v idx len }
+            <:
+            t_SplitInclusive v_T v_P
+          in
+          self, (Core_models.Option.Option_Some res <: Core_models.Option.t_Option (t_Slice v_T))
+          <:
+          (t_SplitInclusive v_T v_P & Core_models.Option.t_Option (t_Slice v_T))
+      in
+      self, hax_temp_output
+      <:
+      (t_SplitInclusive v_T v_P & Core_models.Option.t_Option (t_Slice v_T))
+  }
+
+/// See [`std::slice::SplitN`]
+type t_SplitN (v_T: Type0) (v_P: Type0) = {
+  f_inner:t_Split v_T v_P;
+  f_count:usize
+}
+
+let impl_15__new
+      (#v_T #v_P: Type0)
+      (#[FStar.Tactics.Typeclasses.tcresolve ()] i0: Core_models.Ops.Function.t_Fn v_P v_T)
+      (v: t_Slice v_T)
+      (n: usize)
+      (pred: v_P)
+    : t_SplitN v_T v_P =
+  { f_inner = impl_11__new #v_T #v_P v pred; f_count = n } <: t_SplitN v_T v_P
+
+[@@ FStar.Tactics.Typeclasses.tcinstance]
+let impl_16
+      (#v_T #v_P: Type0)
+      (#[FStar.Tactics.Typeclasses.tcresolve ()] i0: Core_models.Ops.Function.t_Fn v_P v_T)
+    : Core_models.Iter.Traits.Iterator.t_Iterator (t_SplitN v_T v_P) =
+  {
+    f_Item = t_Slice v_T;
+    f_next_pre = (fun (self: t_SplitN v_T v_P) -> true);
+    f_next_post
+    =
+    (fun
+        (self: t_SplitN v_T v_P)
+        (out1: (t_SplitN v_T v_P & Core_models.Option.t_Option (t_Slice v_T)))
+        ->
+        true);
+    f_next
+    =
+    fun (self: t_SplitN v_T v_P) ->
+      let (self: t_SplitN v_T v_P), (hax_temp_output: Core_models.Option.t_Option (t_Slice v_T)) =
+        if self.f_count =. mk_usize 0
+        then
+          self, (Core_models.Option.Option_None <: Core_models.Option.t_Option (t_Slice v_T))
+          <:
+          (t_SplitN v_T v_P & Core_models.Option.t_Option (t_Slice v_T))
+        else
+          if self.f_count =. mk_usize 1
+          then
+            let self:t_SplitN v_T v_P = { self with f_count = mk_usize 0 } <: t_SplitN v_T v_P in
+            let (tmp0: t_Split v_T v_P), (out: Core_models.Option.t_Option (t_Slice v_T)) =
+              impl_11__finish #v_T #v_P self.f_inner
+            in
+            let self:t_SplitN v_T v_P = { self with f_inner = tmp0 } <: t_SplitN v_T v_P in
+            self, out <: (t_SplitN v_T v_P & Core_models.Option.t_Option (t_Slice v_T))
+          else
+            let self:t_SplitN v_T v_P =
+              { self with f_count = self.f_count -! mk_usize 1 } <: t_SplitN v_T v_P
+            in
+            let (tmp0: t_Split v_T v_P), (out: Core_models.Option.t_Option (t_Slice v_T)) =
+              Core_models.Iter.Traits.Iterator.f_next #(t_Split v_T v_P)
+                #FStar.Tactics.Typeclasses.solve
+                self.f_inner
+            in
+            let self:t_SplitN v_T v_P = { self with f_inner = tmp0 } <: t_SplitN v_T v_P in
+            self, out <: (t_SplitN v_T v_P & Core_models.Option.t_Option (t_Slice v_T))
+      in
+      self, hax_temp_output <: (t_SplitN v_T v_P & Core_models.Option.t_Option (t_Slice v_T))
+  }
+
+/// See [`std::slice::RSplit`]
+type t_RSplit (v_T: Type0) (v_P: Type0) = { f_inner:t_Split v_T v_P }
+
+let impl_17__new
+      (#v_T #v_P: Type0)
+      (#[FStar.Tactics.Typeclasses.tcresolve ()] i0: Core_models.Ops.Function.t_Fn v_P v_T)
+      (v: t_Slice v_T)
+      (pred: v_P)
+    : t_RSplit v_T v_P = { f_inner = impl_11__new #v_T #v_P v pred } <: t_RSplit v_T v_P
+
+[@@ FStar.Tactics.Typeclasses.tcinstance]
+let impl_18
+      (#v_T #v_P: Type0)
+      (#[FStar.Tactics.Typeclasses.tcresolve ()] i0: Core_models.Ops.Function.t_Fn v_P v_T)
+    : Core_models.Iter.Traits.Iterator.t_Iterator (t_RSplit v_T v_P) =
+  {
+    f_Item = t_Slice v_T;
+    f_next_pre = (fun (self: t_RSplit v_T v_P) -> true);
+    f_next_post
+    =
+    (fun
+        (self: t_RSplit v_T v_P)
+        (out1: (t_RSplit v_T v_P & Core_models.Option.t_Option (t_Slice v_T)))
+        ->
+        true);
+    f_next
+    =
+    fun (self: t_RSplit v_T v_P) ->
+      let (tmp0: t_Split v_T v_P), (out: Core_models.Option.t_Option (t_Slice v_T)) =
+        impl_11__next_back #v_T #v_P self.f_inner
+      in
+      let self:t_RSplit v_T v_P = { self with f_inner = tmp0 } <: t_RSplit v_T v_P in
+      let hax_temp_output:Core_models.Option.t_Option (t_Slice v_T) = out in
+      self, hax_temp_output <: (t_RSplit v_T v_P & Core_models.Option.t_Option (t_Slice v_T))
+  }
+
+/// See [`std::slice::RSplitN`]
+type t_RSplitN (v_T: Type0) (v_P: Type0) = {
+  f_inner:t_Split v_T v_P;
+  f_count:usize
+}
+
+let impl_19__new
+      (#v_T #v_P: Type0)
+      (#[FStar.Tactics.Typeclasses.tcresolve ()] i0: Core_models.Ops.Function.t_Fn v_P v_T)
+      (v: t_Slice v_T)
+      (n: usize)
+      (pred: v_P)
+    : t_RSplitN v_T v_P =
+  { f_inner = impl_11__new #v_T #v_P v pred; f_count = n } <: t_RSplitN v_T v_P
+
+[@@ FStar.Tactics.Typeclasses.tcinstance]
+let impl_20
+      (#v_T #v_P: Type0)
+      (#[FStar.Tactics.Typeclasses.tcresolve ()] i0: Core_models.Ops.Function.t_Fn v_P v_T)
+    : Core_models.Iter.Traits.Iterator.t_Iterator (t_RSplitN v_T v_P) =
+  {
+    f_Item = t_Slice v_T;
+    f_next_pre = (fun (self: t_RSplitN v_T v_P) -> true);
+    f_next_post
+    =
+    (fun
+        (self: t_RSplitN v_T v_P)
+        (out1: (t_RSplitN v_T v_P & Core_models.Option.t_Option (t_Slice v_T)))
+        ->
+        true);
+    f_next
+    =
+    fun (self: t_RSplitN v_T v_P) ->
+      let (self: t_RSplitN v_T v_P), (hax_temp_output: Core_models.Option.t_Option (t_Slice v_T)) =
+        if self.f_count =. mk_usize 0
+        then
+          self, (Core_models.Option.Option_None <: Core_models.Option.t_Option (t_Slice v_T))
+          <:
+          (t_RSplitN v_T v_P & Core_models.Option.t_Option (t_Slice v_T))
+        else
+          if self.f_count =. mk_usize 1
+          then
+            let self:t_RSplitN v_T v_P = { self with f_count = mk_usize 0 } <: t_RSplitN v_T v_P in
+            let (tmp0: t_Split v_T v_P), (out: Core_models.Option.t_Option (t_Slice v_T)) =
+              impl_11__finish #v_T #v_P self.f_inner
+            in
+            let self:t_RSplitN v_T v_P = { self with f_inner = tmp0 } <: t_RSplitN v_T v_P in
+            self, out <: (t_RSplitN v_T v_P & Core_models.Option.t_Option (t_Slice v_T))
+          else
+            let self:t_RSplitN v_T v_P =
+              { self with f_count = self.f_count -! mk_usize 1 } <: t_RSplitN v_T v_P
+            in
+            let (tmp0: t_Split v_T v_P), (out: Core_models.Option.t_Option (t_Slice v_T)) =
+              impl_11__next_back #v_T #v_P self.f_inner
+            in
+            let self:t_RSplitN v_T v_P = { self with f_inner = tmp0 } <: t_RSplitN v_T v_P in
+            self, out <: (t_RSplitN v_T v_P & Core_models.Option.t_Option (t_Slice v_T))
+      in
+      self, hax_temp_output <: (t_RSplitN v_T v_P & Core_models.Option.t_Option (t_Slice v_T))
+  }
+
+/// See [`std::slice::ChunkBy`]
+type t_ChunkBy (v_T: Type0) (v_P: Type0) = {
+  f_v:t_Slice v_T;
+  f_pred:v_P
+}
+
+let impl_21__new
+      (#v_T #v_P: Type0)
+      (#[FStar.Tactics.Typeclasses.tcresolve ()] i0: Core_models.Ops.Function.t_Fn v_P (v_T & v_T))
+      (v: t_Slice v_T)
+      (pred: v_P)
+    : t_ChunkBy v_T v_P = { f_v = v; f_pred = pred } <: t_ChunkBy v_T v_P
+
+[@@ FStar.Tactics.Typeclasses.tcinstance]
+assume
+val impl_22': #v_T: Type0 -> #v_P: Type0 -> {| i0: Core_models.Ops.Function.t_Fn v_P (v_T & v_T) |}
+  -> Core_models.Iter.Traits.Iterator.t_Iterator (t_ChunkBy v_T v_P)
+
+unfold
+let impl_22
+      (#v_T #v_P: Type0)
+      (#[FStar.Tactics.Typeclasses.tcresolve ()] i0: Core_models.Ops.Function.t_Fn v_P (v_T & v_T))
+     = impl_22' #v_T #v_P #i0
